	\begin{align*}
	Debito={}&Pagato+Sconto\\
	={}&Pagato+\dfrac{Sp\cdot Debito}{100}\\
	Pagato={}&Debito-\dfrac{Sp\cdot Debito}{100}\\
	={}&Debito\left(1-\dfrac{Sp}{100}\right)\\
	Debito={}&\dfrac{Pagato}{1-\dfrac{Sp}{100}}\\
	Debito={}&\dfrac{\mbox{\EUR{171}}}{1-\dfrac{24}{100}}\\
	={}&\mbox{\EUR{225}}
	\end{align*}
Si poteva, riflettendoci sopra, operare in questa maniera:
\[Debito=Pagato+Sconto\]
Quindi se lo sconto è il \SI{24}{\percent} del debito, il pagato è il \SI{76}{\percent}. Quindi
\begin{align*}
	P={}&\dfrac{Pagato}{Debito}\cdot100\\
	76={}&\dfrac{\mbox{\EUR{171}}}{Debito}\cdot 100\\
	Debito={}&\dfrac{\mbox{\EUR{171}}}{76}\cdot 100\\
	={}&\mbox{\EUR{225}}
\end{align*}
